Decompress implementation + example tests

LZ.v
@@ -1,5 +1,5 @@
 From Stdlib Require Import Arith Strings.Byte List Lia.
-Require Import Utils LZ_Matching LZ_Tokens.
+Require Import Utils LZ_Matching LZ_Tokens LZ_Expand.
 Import ListNotations.
 
 Module Impl.
@@ -19,8 +19,16 @@ Module Impl.
   Definition compress (s: list byte): list Token :=
     compress' [] s 0.
 
-  Fixpoint decompress (l : list Token) : list byte := nil. 
+  Fixpoint decompress' (acc : list byte) (l : list Token) : list byte :=
+    match l with
+    | [] => acc
+    | Lit b :: tl => decompress' (acc ++ [b]) tl
+    | Ref len off :: tl => decompress' (expand_ref acc len off) tl
+    end.
 
+  Definition decompress (l : list Token) : list byte :=
+    decompress' [] l.
+  
   Theorem correctness: forall s,
     decompress (compress s) = s.
   Proof.
@@ -32,3 +40,56 @@ Module Impl.
   Admitted.
 
 End Impl.
+
+Section Tests.
+  Import Impl.
+
+  Definition empty : list byte := [].
+  Definition literals : list byte := ["010"%byte; "011"%byte].
+  Definition compressed_literals : list Token := [Lit "010"%byte; Lit "011"%byte].
+  Definition repeating : list byte := [zero; one; one; zero; one; zero; one; one; zero].
+  Definition overlapping : list byte := [zero; one; zero; one; zero; one].
+  Definition compressed_repeating : list Token := [Lit zero; Lit one; Lit one; Lit zero; Lit one; Ref 4 5].
+  Definition compressed_overlapping : list Token := [Lit zero; Lit one; Ref 4 2].
+  
+  Example compress_empty_test :
+    compress empty = [].
+  Proof. reflexivity. Qed.
+  
+  Example decompress_empty_test :
+    decompress [] = empty.
+  Proof. reflexivity. Qed.
+  
+  Example compress_literals_test :
+    compress literals = compressed_literals.
+  Proof. reflexivity. Qed.
+  
+  Example decompress_literals_test :
+    decompress compressed_literals = literals.
+  Proof. reflexivity. Qed.
+  
+  Example compress_repetition_test :
+    compress repeating = compressed_repeating.
+  Proof. reflexivity. Qed.
+  
+  Example decompress_overlap_test :
+    decompress compressed_overlapping = overlapping.
+  Proof. reflexivity. Qed.
+  
+  Example correctness_empty :
+    decompress (compress empty) = empty.
+  Proof. reflexivity. Qed.
+  
+  Example correctness_simple :
+    decompress (compress [zero]) = [zero].
+  Proof. reflexivity. Qed.
+  
+  Example correctness_repeating :
+    decompress (compress repeating) = repeating.
+  Proof. reflexivity. Qed.
+  
+  Example correctness_overlapping :
+    decompress (compress overlapping) = overlapping.
+  Proof. reflexivity. Qed.
+
+End Tests.
